refactor: Update to coq-base

plugins/exec/coqbytestring.ml
@@ -1,0 +1,65 @@
+(* FreeSpec
+ * Copyright (C) 2018–2020 ANSSI
+ *
+ * Contributors:
+ * 2020 Thomas Letan <thomas.letan@ssi.gouv.fr>
+ *
+ * This program is free software: you can redistribute it and/or modify
+ * it under the terms of the GNU General Public License as published by
+ * the Free Software Foundation, either version 3 of the License, or
+ * (at your option) any later version.
+ *
+ * This program is distributed in the hope that it will be useful,
+ * but WITHOUT ANY WARRANTY; without even the implied warranty of
+ * MERCHANTABILITY or FITNESS FOR A PARTICULAR PURPOSE.  See the
+ * GNU General Public License for more details.
+ *
+ * You should have received a copy of the GNU General Public License
+ * along with this program. If not, see <http://www.gnu.org/licenses/>.
+ *)
+
+open Coqbase
+open Constr
+open Query
+open Coqbyte
+open Utils
+
+let coqbytestr_nil = Ind.Bytestring.mkConstructor "bytes_nil"
+let coqbytestr_cons x rst =
+  mkApp
+    (Ind.Bytestring.mkConstructor "bytes_cons", Array.of_list [rst])
+
+let rec coqbytestr_fold_left f trm acc =
+  let (c, args) = app_full trm in
+  match (Ind.Bytestring.constructor_of c, args) with
+  | (Some Bytes_nil, []) -> acc
+  | (Some Bytes_cons, [coqx; coqrst]) ->
+     coqbytestr_fold_left f coqrst (f acc coqx)
+  | _ -> raise (UnsupportedTerm "coqbytestr_fold_left: not a bytestring")
+
+let coqbytestr_iteri f =
+  let rec aux idx trm =
+    let (c, args) = app_full trm in
+    match (Ind.Bytestring.constructor_of c, args) with
+    | (Some Bytes_nil, []) -> ()
+    | (Some Bytes_cons, [coqx; coqrst]) ->
+       f idx coqx;
+       aux (idx + 1) coqrst
+    | _ -> raise (UnsupportedTerm "coqbytestr_iteri: not a bytestring")
+  in aux 0
+
+let bytestring_of_coqbytestring trm =
+  let size = coqbytestr_fold_left (fun x _ -> x + 1) trm 0 in
+  let buffer = Bytes.create size in
+  let aux idx c = Bytes.set buffer idx (char_of_coqbyte c) in
+  let _ = coqbytestr_iteri aux trm in
+  Bytestring.of_string (Bytes.to_string buffer)
+
+let bytestring_to_coqbytestring b =
+  Seq.fold_left
+    (fun cont c next -> cont (coqbytestr_cons (char_to_coqbyte c) next))
+    (fun x -> x)
+    (String.to_seq (Bytestring.to_string b))
+    coqbytestr_nil
+
+let coqbytestring_t = Ind.Bytestring.mkInductive
