plugins/exec/coqi63.ml
@@ -18,19 +18,24 @@
  * along with this program. If not, see <http://www.gnu.org/licenses/>.
  *)
 
-open Freespec_exec.Coqstr
-open Freespec_exec.Extends
-open Freespec_exec.Coqunit
+open Query
+open Utils
 
-let path = "freespec.stdlib.console"
+let int_of_coqint coqint =
+  match Constr.kind coqint with
+  | Constr.Int i -> snd (Uint63.to_int2 i)
+  | _ -> raise (UnsupportedTerm "Not a native integer")
 
-let install_interface =
-  let scan = function
-    | [] -> bytes_to_coqbytes (Bytes.of_string @@ read_line ())
-    | _ -> assert false in
-  let echo = function
-    | [str] -> print_bytes (bytes_of_coqbytes str);
-               flush stdout;
-               coqtt
-    | _ -> assert false in
-  register_interface path [("Scan", scan); ("Echo", echo)]
+let int_to_coqint v = Constr.(of_kind (Int (Uint63.of_int v)))
+
+let int_of_coqi63 trm =
+  let (c, args) = app_full trm in
+  match (Ind.I63.constructor_of c, args) with
+  | (Some Mk_i63, [trm]) -> int_of_coqint trm
+  | _ -> raise (UnsupportedTerm "int_of_coqi63")
+
+let int_to_coqi63 n =
+  let trm = int_to_coqint n in
+  Constr.mkApp (Ind.I63.mkConstructor "mk_i63", Array.of_list [trm])
+
+let coqi63_t = Ind.I63.mkInductive
