theories/Stdlib/env.mli
@@ -1,0 +1,4 @@
+open Coqbase
+
+val getenv : Bytestring.t -> Bytestring.t option [@@impure]
+val setenv : Bytestring.t -> Bytestring.t -> unit [@@impure]
