theories/Stdlib/files.mli
@@ -1,0 +1,20 @@
+open Coqbase
+
+type file_descriptor
+
+type file_err = FileErr of int
+
+type file_flag =
+  | O_RDONLY
+  | O_WRONLY
+  | O_RDWR
+
+val stdin : file_descriptor
+val stdout : file_descriptor
+
+val openfile : Bytestring.t -> (file_err, file_descriptor) Sum.t [@@impure]
+val read : file_descriptor -> int -> (file_err, Bytestring.t) Sum.t [@@impure]
+val read_line : file_descriptor -> (file_err, Bytestring.t) Sum.t [@@impure]
+val fsize : file_descriptor -> (file_err, int) Sum.t [@@impure]
+val write : file_descriptor -> Bytestring.t -> int -> int -> (file_err, int) Sum.t [@@impure]
+val close : file_descriptor -> (file_err, unit) Sum.t [@@impure]
