theories/Core/Impure.v
@@ -29,8 +29,8 @@
     <<https://github.com/whitequark/unfork#introduction>>). *)
 
 From Coq Require Import Program Setoid Morphisms.
-From Prelude Require Import All.
-From FreeSpec.Core Require Import Interface.
+From Base Require Export State.
+From FreeSpec.Core Require Export Interface.
 
 #[local]
 Open Scope signature_scope.
@@ -120,24 +120,29 @@ Next Obligation.
     now apply H with (β := x).
 Qed.
 
-#[program]
-Instance impure_Equality : Equality (impure i α).
+Instance impure_EquProp : EquProp (impure i α) :=
+  { equal := impure_equiv }.
+
+Instance impure_EquPropL : EquPropL (impure i α) := {}.
 
 #[global]
-Opaque impure_Equality.
+Opaque impure_EquProp.
 
-(* FIXME[0]: This works because coq-prelude provides a default [Equality]
-   instance for any type is [eq].  Since [b] is universally quantified, there is
-   no specific instance to pick expect this one, and therefore the instance of
-   Equality for [a -> b] is [forall x, f x = g x], which is exactly what we
-   need. *)
 #[program]
-Instance request_then_Proper : Proper (eq ==> 'equal ==> 'equal) (@request_then i α β).
+Instance request_then_Proper {i α β} (e : i β)
+  : EquMorphism (@request_then i α β e).
 
 Next Obligation.
   add_morphism_tactic.
-  intros x f g equ.
-  now constructor.
+  intros f g equ.
+  constructor.
+  intros y.
+  specialize (equ y).
+  inversion equ; subst.
+  + reflexivity.
+  + constructor.
+    intros z.
+    apply equ0.
 Qed.
 
 (** ** Monad Instances *)
@@ -152,74 +157,62 @@ Fixpoint impure_bind {i α β} (p : impure i α) (f : α -> impure i β) : impur
   end.
 
 #[program]
-Instance impure_bind_Proper_1 : Proper (eq ==> 'equal ==> 'equal) (@impure_bind i α β).
+Instance impure_bind_Proper {i α β} : EquMorphism (@impure_bind i α β).
 
 Next Obligation.
   add_morphism_tactic.
-  intros p f g equf.
-  induction p.
-  + apply equf.
-  + constructor.
-    intros sem.
-    apply H.
-Qed.
-
-#[program]
-Instance impure_bind_Proper_2 : Proper ('equal ==> eq ==> 'equal) (@impure_bind i α β).
-
-Next Obligation.
-  add_morphism_tactic.
-  intros p q equp f.
-  induction equp.
-  + reflexivity.
+  intros x y equ1 f g equ2.
+  induction equ1.
+  + apply equ2.
   + cbn.
     constructor.
+    intros x.
     apply H.
 Qed.
 
 Ltac change_request_then :=
   match goal with
-  | |- request_then ?e ?f == request_then ?e ?g =>
+  | |- request_then ?e ?f === request_then ?e ?g =>
     let R := fresh "R" in
-    assert (R: f == g); [ intros ?x | rewrite R; clear R ]
+    assert (R: f === g); [ intros ?x | rewrite R; clear R ]
   end.
 
 Ltac change_impure_bind :=
   match goal with
-  | |- impure_bind ?e ?f == impure_bind ?e ?g =>
+  | |- impure_bind ?e ?f === impure_bind ?e ?g =>
     let R := fresh "R" in
-    assert (R: f == g); [ intros ?x | now rewrite R ]
+    assert (R: f === g); [ intros ?x | now rewrite R ]
   end.
 
-Lemma impure_bind_local {i α} (p : impure i α) : impure_bind p (fun x => local x) == p.
+Lemma impure_bind_local {i α} (p : impure i α)
+  : impure_bind p (fun x => local x) === p.
 
 Proof.
   induction p.
   + reflexivity.
   + cbn.
-    change_request_then; [| reflexivity ].
+    change_request_then; [ | reflexivity ].
     now rewrite H.
 Qed.
 
 Lemma impure_bind_assoc {i α β δ}
   (p : impure i α) (f : α -> impure i β) (g : β -> impure i δ)
-  : impure_bind (impure_bind p f) g == impure_bind p (fun x => impure_bind (f x) g).
+  : impure_bind (impure_bind p f) g === impure_bind p (fun x => impure_bind (f x) g).
 
 Proof.
-  induction p; [reflexivity |].
+  induction p; [reflexivity | ].
   cbn.
-  change_request_then; [| reflexivity ].
+  change_request_then; [ | reflexivity ].
   now rewrite H.
 Qed.
 
-(* see FIXME[0] *)
 Definition impure_map {i α β} (f : α -> β) (p : impure i α) : impure i β :=
   impure_bind p (fun x => local (f x)).
 
-#[program]
-Instance impure_map_Proper : Proper ('equal ==> 'equal ==> 'equal) (@impure_map i α β).
+Instance impure_map_Proper {i α β}
+  : EquMorphism (@impure_map i α β).
 
-Next Obligation.
+Proof.
   add_morphism_tactic.
   intros f g equf p q equp.
   unfold impure_map.
@@ -228,10 +221,12 @@ Next Obligation.
   now rewrite equf.
 Qed.
 
-#[program]
 Instance impure_Functor : Functor (impure i) :=
   { map := @impure_map i
   }.
+
+#[program]
+Instance impure_FunctorL : FunctorL (impure i) := {}.
 
 Next Obligation.
   unfold impure_map.
@@ -250,7 +245,7 @@ Definition impure_apply {i α β} (p : impure i (α -> β)) (q : impure i α) : 
   impure_bind p (fun f => map f q).
 
 #[program]
-Instance impure_apply_Proper : Proper ('equal ==> 'equal ==> 'equal) (@impure_apply i α β).
+Instance impure_apply_Proper {i α β} : EquMorphism (@impure_apply i α β).
 
 Next Obligation.
   add_morphism_tactic.
@@ -262,64 +257,62 @@ Next Obligation.
   now rewrite equ2.
 Qed.
 
-#[program, universes(polymorphic)]
 Instance impure_Applicative : Applicative (impure i) :=
   { pure := @impure_pure i
   ; apply := @impure_apply i
   }.
 
-Next Obligation.
-  unfold impure_apply, impure_pure, impure_bind.
-  now rewrite functor_identity.
-Defined.
+#[refine]
+Instance impure_ApplicativeL : ApplicativeL (impure i) := {}.
 
-Next Obligation.
-  unfold impure_apply, impure_pure; cbn.
-  unfold impure_map.
-  repeat rewrite impure_bind_assoc.
-  change_impure_bind; cbn.
-  repeat rewrite impure_bind_assoc.
-  change_impure_bind; cbn.
-  repeat rewrite impure_bind_assoc.
-  now change_impure_bind.
-Defined.
-
-Next Obligation.
-  reflexivity.
+Proof.
+  + intros a Ha Ha' v.
+    induction v; [ reflexivity | ].
+    cbn.
+    constructor.
+    intros x.
+    apply H.
+  + intros a b c Hc Hc' u v w.
+    cbn.
+    unfold impure_apply, impure_pure; cbn.
+    unfold impure_map.
+    repeat rewrite impure_bind_assoc.
+    cbn.
+    change_impure_bind; cbn.
+    repeat rewrite impure_bind_assoc.
+    change_impure_bind; cbn.
+    repeat rewrite impure_bind_assoc.
+    now change_impure_bind.
+  + reflexivity.
+  + reflexivity.
+  + reflexivity.
 Qed.
 
-Next Obligation.
-  reflexivity.
-Qed.
-
-Next Obligation.
-  reflexivity.
-Qed.
+Instance impure_Monad (i : interface) : Monad (impure i) :=
+  { bind := @impure_bind i }.
 
 #[program]
-Instance impure_Monad (i : interface) : Monad (impure i) :=
-  { bind := @impure_bind i
-  }.
+Instance impure_MonadL (i : interface) : MonadL (impure i).
 
 Next Obligation.
   reflexivity.
-Defined.
+Qed.
 
 Next Obligation.
   now rewrite impure_bind_local.
-Defined.
+Qed.
 
 Next Obligation.
   now rewrite impure_bind_assoc.
-Defined.
+Qed.
 
 Next Obligation.
   now change_impure_bind.
-Defined.
+Qed.
 
 Next Obligation.
   reflexivity.
-Defined.
+Qed.
 
 (** ** Defining Impure Computations *)
 
@@ -337,7 +330,7 @@ Defined.
     that it has to provide at least [i]'s primitives.  *)
 
 Definition request `{Provide ix i} {α} (e : i α) : impure ix α :=
-  request_then (inj_p e) (fun* x => pure x).
+  request_then (inj_p e) (fun x => pure x).
 
 (** Note: there have been attempts to turn [request] into a typeclass
     function (to seamlessly use [request] with a [MonadTrans] instance such as
@@ -350,9 +343,6 @@ Definition request `{Provide ix i} {α} (e : i α) : impure ix α :=
     The <<coq-prelude>> provides notations (inspired by the do notation of
     Haskell) to write monadic functions more easily.  These notations live
     inside the [monad_scope]. *)
-
-Declare Scope impure_scope.
-Bind Scope monad_scope with impure.
 
 Instance store_monad_state (s : Type) (ix : interface) `{Provide ix (STORE s)}
   : MonadState s (impure ix) :=
