theories/Core/Extraction.v
@@ -1,0 +1,3 @@
+From FreeSpec.Core Require Import All.
+
+Extraction Inline impure_Applicative.
