theories/Stdlib/Raise.v
@@ -1,12 +1,10 @@
 From FreeSpec.Core Require Import All.
 
 Class Into (α β : Type) :=
-  { into : α -> β
-  }.
+  { into : α -> β }.
 
 Instance refl_Into (α : Type) : Into α α :=
-  { into := fun x => x
-  }.
+  { into := fun x => x }.
 
 Inductive RAISE (α : Type) : interface :=
 | Raise {β} (x : α) : RAISE α β.
@@ -17,11 +15,10 @@ Definition raise `{Into δ α, Provide ix (RAISE α)} {β} (x : δ) : impure ix 
   request (Raise (into x)).
 
 Definition try `{Into δ α, Provide ix (RAISE α)} {β} (p : impure ix (δ + β)) : impure ix β :=
-  do let* res := p in
-     match res with
-     | inl e => raise e
-     | inr x => pure x
-     end
+  let* res := p in
+  match res with
+  | inl e => raise e
+  | inr x => pure x
   end.
 
 Fixpoint with_raise {ix α β} (p : impure (ix + RAISE α) β) : impure ix (α + β) :=
@@ -32,11 +29,10 @@ Fixpoint with_raise {ix α β} (p : impure (ix + RAISE α) β) : impure ix (α +
   end.
 
 Fixpoint recover {ix α β} (p : impure (ix + RAISE α) β) (h : α -> impure ix β) : impure ix β :=
-  do let* res := with_raise p in
-     match res with
-     | inl e => h e
-     | inr x => pure x
-     end
+  let* res := with_raise p in
+  match res with
+  | inl e => h e
+  | inr x => pure x
   end.
 
 Declare Scope raise_scope.
@@ -44,4 +40,10 @@ Declare Scope raise_scope.
 Notation "'recover' p 'with'  v 'of' t '=>' h 'end'" :=
   (recover p (fun (v : t) => h)) : raise_scope.
 
+#[global]
 Open Scope raise_scope.
+
+Definition halt_on_error {ix α} (p : impure (ix + RAISE α) unit) : impure ix unit :=
+  recover p
+  with _ of α => pure tt
+  end.
